\subsubsection{三角}
\paragraph{$\blacksquare$ 复分析欧拉公式}
\noindent \\
$$e^{ix}=\cos x+i\sin x$$（可简单导出棣莫弗定理）
\paragraph{$\blacksquare$ 和差公式}
\noindent \\
$\sin(\alpha \pm \beta )=\sin \alpha \cos \beta \pm \cos \alpha \sin \beta$~~~~~~~~
$\cos(\alpha \pm \beta )=\cos \alpha \cos \beta \mp \sin \alpha \sin \beta$\\
$\tan(\alpha \pm \beta )={\frac{\tan \alpha \pm \tan \beta }{1\mp \tan \alpha \tan \beta }}$\\
\paragraph{$\blacksquare$ 和差化积}
\noindent \\
$\sin \alpha +\sin \beta =2\sin {\frac  {\alpha +\beta }{2}}\cos {\frac  {\alpha -\beta }{2}}$~~~~~~~~
$\cos \alpha +\cos \beta =2\cos {\frac  {\alpha +\beta }{2}}\cos {\frac  {\alpha -\beta }{2}}$\\
$\cos \alpha -\cos \beta =-2\sin {\alpha +\beta  \over 2}\sin {\alpha -\beta  \over 2}$~~~~~~~~
$\sin \alpha -\sin \beta =2\cos {\alpha +\beta  \over 2}\sin {\alpha -\beta  \over 2}$\\
\paragraph{$\blacksquare$ 积化和差}
\noindent \\
$\sin \alpha \sin \beta =\frac{\cos(\alpha -\beta )-\cos(\alpha +\beta )}{2}$~~~~~~~~
$\cos \alpha \cos \beta =\frac{\cos(\alpha -\beta )+\cos(\alpha +\beta )}{2}$\\
$\sin \alpha \cos \beta =\frac{\cos(\alpha +\beta )+\cos(\alpha -\beta )}{2}$~~~~~~~~
$\cos \alpha \sin \beta =\frac{\cos(\alpha +\beta )-\cos(\alpha -\beta )}{2}$\\
\paragraph{$\blacksquare$ 二、三、$n$倍角（切比雪夫）}
\noindent \\
$\sin 2\theta =2\sin \theta \cos \theta =\frac{2\tan \theta}{1+\tan ^2 \theta}$\\
$\cos 2\theta =\cos ^2 \theta -\sin ^2 \theta =2\cos ^2 \theta -1=1-2\sin ^2 \theta=\frac{1-\tan ^2 \theta}{1+\tan ^2 \theta}$\\
$\tan 2\theta =\frac{2\tan \theta}{1-\tan ^2 \theta}=\frac{1}{1-\tan \theta}-\frac{1}{1+\tan \theta}$\\
$\sin 3\theta =3\sin \theta-4\sin ^3 \theta$~~~~~~~~
$\cos 3\theta=4\cos ^3 \theta-3\cos \theta$~~~~~~~~
$\tan 3\theta=\frac{3\tan \theta -\tan ^3 \theta}{1-3\tan ^2 \theta}$\\
$\begin{aligned} \sin n\theta &=\sum _{{k=0}}^{n}{\binom  {n}{k}}\cos ^{k}\theta \,\sin ^{{n-k}}\theta \,\sin \left[{\frac  {1}{2}}(n-k)\pi \right] \\&=\sin \theta \sum _{{k=0}}^{{\lfloor {\frac  {n-1}{2}}\rfloor }}(-1)^{k}{\binom  {n-1-k}{k}}(2\cos \theta )^{n-1-2k} \end{aligned}$\\
$\begin{aligned} \cos n\theta &=\sum _{{k=0}}^{n}{\binom  {n}{k}}\cos ^{k}\theta \,\sin ^{{n-k}}\theta \,\cos \left[{\frac  {1}{2}}(n-k)\pi \right] \\&={\frac  {1}{2}}\sum _{{k=0}}^{{\lfloor {\frac  {n}{2}}\rfloor }}(-1)^{k}{\frac  {n}{n-k}}{\binom  {n-k}{k}}(2\cos \theta )^{n-2k} \end{aligned}$\\
\paragraph{$\blacksquare$ 二、三次降幂}
\noindent \\
$\sin ^{2}\theta ={\frac  {1-\cos 2\theta }{2}}$~~~~
$\cos ^{2}\theta ={\frac  {1+\cos 2\theta }{2}}$~~~~
$\sin ^{3}\theta ={\frac  {3\sin \theta -\sin 3\theta }{4}}$~~~~
$\cos ^{3}\theta ={\frac  {3\cos \theta +\cos 3\theta }{4}}$\\
\paragraph{$\blacksquare$ 万能公式}
\noindent \\
$t=\tan \frac{\theta}{2}$~~~$\Rightarrow$~~~
$\sin \theta = \frac{2t}{1+t^2}$~~~~~~
$\cos \theta = \frac{1-t^2}{1+t^2}$~~~~~~~
$\sin \theta = \frac{2t}{1-t^2}$~~~~~~
$\mathrm{d}x=\frac{2}{1+t^2}\mathrm{d}t$\\
\paragraph{$\blacksquare$ 连乘}
\noindent \\
${\displaystyle \prod _{{k=0}}^{{n-1}}\cos 2^{k}\theta ={\frac  {\sin 2^{n}\theta }{2^{n}\sin \theta }}}$~~~
${\displaystyle \prod _{{k=0}}^{{n-1}}\sin \left(x+{\frac  {k\pi }{n}}\right)={\frac  {\sin nx}{2^{{n-1}}}}}$\\
${\displaystyle \prod _{{k=1}}^{{n-1}}\sin \left({\frac  {k\pi }{n}}\right)={\frac  {n}{2^{{n-1}}}}}$~~~
${\displaystyle \prod _{{k=1}}^{{n-1}}\sin \left({\frac  {k\pi }{2n}}\right)={\frac  {{\sqrt  {n}}}{2^{{n-1}}}}}$~~~
${\displaystyle \prod _{{k=1}}^{{n}}\sin \left({\frac  {k\pi }{2n+1}}\right)={\frac  {{\sqrt  {2n+1}}}{2^{n}}}}$\\
${\displaystyle \prod _{{k=1}}^{{n-1}}\cos \left({\frac  {k\pi }{n}}\right)={\frac  {\sin {\frac  {n\pi }{2}}}{2^{{n-1}}}}}$~~~
${\displaystyle \prod _{{k=1}}^{{n-1}}\cos \left({\frac  {k\pi }{2n}}\right)={\frac  {{\sqrt  {n}}}{2^{{n-1}}}}}$~~~
${\displaystyle \prod _{{k=1}}^{n}\cos \left({\frac  {k\pi }{2n+1}}\right)={\frac  {1}{2^{n}}}}$\\
${\displaystyle \prod _{{k=1}}^{{n-1}}\tan \left({\frac  {k\pi }{n}}\right)={\frac  {n}{\sin {\frac  {n\pi }{2}}}}}$~~~
${\displaystyle \prod _{{k=1}}^{{n-1}}\tan \left({\frac  {k\pi }{2n}}\right)=1}$~~~
${\displaystyle \prod _{{k=1}}^{n}\tan {\frac  {k\pi }{2n+1}}={\sqrt  {2n+1}}}$\\
\paragraph{$\blacksquare$ 其它}
\noindent \\
$x+y+z=n\pi \Rightarrow \tan x+\tan y+\tan z=\tan x \tan y \tan z$\\
$x+y+z=n\pi +\frac{\pi}{2} \Rightarrow \cot x+\cot y+\cot z=\cot x \cot y \cot z$\\
$x+y+z=\pi \Rightarrow \sin 2x+\sin 2y+\sin 2z=4\sin x\sin y\sin z$\\
$\sin(x+y)\sin(x-y)=\sin ^{2}{x}-\sin ^{2}{y}=\cos ^{2}{y}-\cos ^{2}{x}$\\
$\cos(x+y)\cos(x-y)=\cos ^{2}{x}-\sin ^{2}{y}=\cos ^{2}{y}-\sin ^{2}{x}$

%\subsubsection{数列}

\subsubsection{级数}
\paragraph{$\blacksquare$ 泰勒级数}
\noindent \\
$$f(x)=\sum _{n=0}^{\infty }{\frac {f^{(n)}(a)}{n!}}(x-a)^{n}$$
${\displaystyle {\frac {1}{1-x}}=\sum _{n=0}^{\infty }x^{n}\quad \forall x:\left|x\right|<1}$~~~~~~~~~
${\displaystyle (1+x)^{\alpha }=\sum _{n=0}^{\infty }\binom{\alpha}{n} x^{n}\quad \forall x:\left|x\right|<1,\forall \alpha \in \mathbb {C}}$\\
${\displaystyle e^{x}=\sum _{n=0}^{\infty }{\frac {x^{n}}{n!}}\quad \forall x}$\\
${\displaystyle \ln(1+x)=\sum _{n=1}^{\infty }{\frac {(-1)^{n+1}}{n}}x^{n}\quad \forall x:\left| x\right| \leq 1}$~~~~
${\displaystyle \ln(1-x)=-\sum _{n=1}^{\infty }{\frac {x^n}{n}}\quad \forall x:\left| x\right| \leq 1}$\\
${\displaystyle \sin x=\sum _{n=0}^{\infty }{\frac {(-1)^{n}}{(2n+1)!}}x^{2n+1}\quad \forall x}$~~~~~~~~~~~~~~
${\displaystyle \cos x=\sum _{n=0}^{\infty }{\frac {(-1)^{n}}{(2n)!}}x^{2n}\quad \forall x}$\\
${\displaystyle \tan x=\sum _{n=1}^{\infty }{\frac {B_{2n}4^{n}(4^{n}-1)}{(2n)!}}x^{2n-1}\quad \forall x:\left|x\right|<{\frac {\pi }{2}}}$\\
${\displaystyle \arcsin x=\sum _{n=0}^{\infty }{\frac {(2n)!}{4^{n}(n!)^{2}(2n+1)}}x^{2n+1}\quad \forall x:\left|x\right|<1}$\\
${\displaystyle \arctan x=\sum _{n=0}^{\infty }{\frac {(-1)^{n}}{2n+1}}x^{2n+1}\quad \forall x:\left|x\right|<1}$\\
${\displaystyle \sinh x=\sum _{n=0}^{\infty }{\frac {1}{(2n+1)!}}x^{2n+1}\quad \forall x}$~~~~~~~~
${\displaystyle \cosh x=\sum _{n=0}^{\infty }{\frac {1}{(2n)!}}x^{2n}\quad \forall x}$

\subsubsection{导数}
\paragraph{$\blacksquare$ 几个导数}
\noindent \\
$(\tan x)'=\sec ^2 x$~~~
$(\arctan x)'=\frac{1}{1+x^2}$~~~
$(\arcsin x)'=\frac{1}{\sqrt{1-x^2}}$~~~
$(\arccos x)'=-\frac{1}{\sqrt{1-x^2}}$\\
$(\sinh x)'=\cosh x=\frac{e^x+e^{-x}}{2}$~~~~
$(\cosh x)'=\sinh x=\frac{e^x-e^{-x}}{2}$
\paragraph{$\blacksquare$ 高阶导数}
\noindent \\
（莱布尼茨公式）
$$(uv)^{(n)}=\sum _{{k=0}}^{n}{\binom{n}{k} u^{(n-k)} v^{(k)}}$$
${\displaystyle (x^a)^{(n)}=x^{a-n} \prod _{{k=0}}^{{n-1}} (a-k)}$~~~~~~~~
$(\frac{1}{x})^{(n)}=(-1)^n\frac{n!}{x^{n+1}}$\\
$(a^x)^{(n)}=a^x \ln ^n a~(a>0)$~~~~~~~~
$(\ln x)^{(n)}=(-1)^{n-1} \frac{(n-1)!}{x^n}$\\
$(\sin (kx+b))^{(n)}=k^n \sin (kx+b+\frac{n\pi}{2})$~~~~
$(\cos (kx+b))^{(n)}=k^n \cos (kx+b+\frac{n\pi}{2})$
\subsubsection{积分表}
\input{Template/integrals.tex}
