\def\Subset#1#2{ \bigg\{{#1 \atop #2} \bigg\}}
\def\subset#1#2{ \big\{{#1 \atop #2} \big\}}
\def\Cycle#1#2{ \bigg[{#1 \atop #2} \bigg]}
\def\cycle#1#2{ \big[{#1 \atop #2} \big]}

$$f(x)=\sum _{n=0}^{\infty }{\frac {f^{(n)}(a)}{n!}}(x-a)^{n}$$
${\displaystyle {1 \over 1 - x}=\sum_{i=0}^\infty x^i}$~~~~
${\displaystyle {1 \over 1 - c x}=\sum_{i=0}^\infty c^i x^i}$~~~~
${\displaystyle {1 \over 1 - x^n}=\sum_{i=0}^\infty x^{ni}}$~~~~
${\displaystyle {x \over (1 - x)^2}=\sum_{i=0}^\infty i x^i}$\\
${\displaystyle\sum_{k=0}^n {n \brace k} {k! z^k \over (1-z)^{k+1}}=\sum_{i=0}^\infty i^n x^i}$~~~~~~~~~~~~~~~~~~~~~
${\displaystyle e^x=\sum_{i=0}^\infty {x^i \over i!}}$\\
${\displaystyle \ln (1 + x)=\sum_{i=1}^\infty (-1)^{i+1} {x^i \over i}}$~~~~~~~~~~~~~~~~~~~~~~~~~~~
${\displaystyle \ln {1 \over 1 - x}=\sum_{i=1}^\infty {x^i \over i}}$\\
${\displaystyle \sin x=\sum_{i=0}^\infty (-1)^i {x^{2i+1} \over (2i+1)!}}$~~~~~~~~~~~~~~~~~~~~~~~~~~~~
${\displaystyle \cos x=\sum_{i=0}^\infty (-1)^i {x^{2i} \over (2i)!} }$\\
${\displaystyle \tan^{-1} x=\sum_{i=0}^\infty (-1)^i {x^{2i+1} \over (2i+1)} }$~~~~~~~~~~~~~~~~~~~~~~~~~
${\displaystyle (1+x)^n=\sum_{i=0}^\infty {n \choose i} x^i }$\\
${\displaystyle {1 \over (1-x)^{n+1}}=\sum_{i=0}^\infty {i+ n \choose i} x^i }$~~~~~~~~~~~~~~~~~~~~~~~~~
${\displaystyle {x \over e^x - 1}=\sum_{i=0}^\infty {b_i x^i \over i!} }$\\
${\displaystyle {1 \over 2x}(1 - \sqrt{1-4x})=\sum_{i=0}^\infty {1 \over i+1}{2i \choose i}x^i }$~~~~~~~~~~~~~~
${\displaystyle {1 \over \sqrt{1-4x}}=\sum_{i=0}^\infty {2i \choose i}x^i }$\\
${\displaystyle {1 \over \sqrt{1-4x}}\left({1 - \sqrt{1-4x} \over 2x}\right)^n=\sum_{i=0}^\infty {2i+n \choose i}x^i }$~~~
${\displaystyle {1 \over 1-x}\ln{1 \over 1- x}=\sum_{i=1}^\infty H_i x^i}$\\
${\displaystyle {1 \over 2}\left(\ln{1 \over 1- x}\right)^2=\sum_{i=2}^\infty {H_{i-1} x^i \over i}}$~~~~~~~~~~~~~~~~~~~~~~~~
${\displaystyle {x \over 1 - x - x^2}=\sum_{i=0}^\infty F_i x^i}$\\
${\displaystyle {F_n x \over 1 - (F_{n-1} + F_{n+1})x - (-1)^n x^2}=\sum_{i=0}^\infty F_{ni} x^i.}$\\
${\displaystyle {1 \over (1-x)^{n+1}}\ln{1 \over 1- x} = \sum_{i=0}^\infty (H_{n+i} - H_n) {n+i \choose i} x^i, \left({1 \over x}\right)^{\overline{-n}} = \sum_{i=0}^\infty \Subset i n x^i}$\\
${\displaystyle x^{\overline{n}} = \sum_{i=0}^\infty \Cycle n i x^i, (e^x - 1)^n = \sum_{i=0}^\infty \Subset i n {n! x^i \over i!}}$\\
${\displaystyle \left(\ln {1 \over 1 -x}\right)^n = \sum_{i=0}^\infty \Cycle i n {n! x^i \over i!}, x \cot x = \sum_{i=0}^\infty {(-4)^i b_{2i} x^{2i} \over (2i)!}}$\\
${\displaystyle \tan x = \sum_{i=1}^\infty (-1)^{i-1}{2^{2i} (2^{2i} - 1) b_{2i} x^{2i-1} \over (2i)!}, \zeta(x) = \sum_{i=1}^\infty {1 \over i^x}}$\\
${\displaystyle {1 \over \zeta(x)} = \sum_{i=1}^\infty {\mu(i) \over i^x}, {\zeta(x-1) \over \zeta(x)} = \sum_{i=1}^\infty {\phi(i) \over i^x}}$\\